src/trusted_code/k8s_io/client_go/kubernetes.v
@@ -1,5 +1,7 @@
 From New.golang Require Import defn.
+Require Export New.code.k8s_io.client_go.kubernetes.typed.apps.v1.
 Require Export New.code.k8s_io.client_go.kubernetes.typed.core.v1.
+Module apps_v1 := code.k8s_io.client_go.kubernetes.typed.apps.v1.v1.
 Module core_v1 := code.k8s_io.client_go.kubernetes.typed.core.v1.v1.
 
 Module kubernetes.
@@ -9,8 +11,23 @@ Context {ext : ffi_syntax} {go_gctx : GoGlobalContext}.
 Definition clientsetType : go.type :=
   go.Named "k8s.io/client-go/kubernetes.Clientset"%go [].
 
+Definition appsV1ClientType : go.type :=
+  apps_v1.AppsV1Client.
+
 Definition coreV1ClientType : go.type :=
   core_v1.CoreV1Client.
+
+(* Trusted Go equivalent:
+
+   func (c *Clientset) AppsV1() appsv1.AppsV1Interface {
+       var client *appsv1.AppsV1Client
+       return client
+   }
+*)
+Definition Clientset__AppsV1ⁱᵐᵖˡ : val :=
+  λ: "c" <>,
+    exception_do (let: "c" := (GoAlloc (go.PointerType clientsetType) "c") in
+    return: (#(interface.mk_ok (go.PointerType appsV1ClientType) (#null)))).
 
 (* Trusted Go equivalent:
 
